src/impl/TLS13.Impl.Serializer.fsti
@@ -4,8 +4,11 @@ module TLS13.Impl.Serializer
 
 open Pulse.Lib.Pervasives
 open Pulse.Lib.Array.PtsTo
+open Pulse.Lib.Box { box }
 
 module B = TLS13.Bytes
+module Box = Pulse.Lib.Box
+module CL = TLS13.ConnectionLog
 module CS = TLS13.Spec.ConnectionState
 module L = TLS13.Impl.Messages
 module M = TLS13.Messages
@@ -14,6 +17,7 @@ module SZ = FStar.SizeT
 module T = TLS13.Types
 module U16 = FStar.UInt16
 module U8 = FStar.UInt8
+module V = Pulse.Lib.Vec
 module WS = TLS13.Wire.Spec
 
 (**
@@ -77,6 +81,202 @@ fn build_supported_client_hello_localhost
           pts_to out out_bytes **
           pure (B.length out_bytes == SZ.v out_len /\
                (ok ==> SZ.v out_len >= 130))
+
+fn serialize_client_hello_from_start
+  (#start: erased CS.handshake_start)
+  (#ch: erased M.client_hello)
+  (start_random: V.vec U8.t)
+  (start_server_name: V.vec U8.t)
+  (start_server_name_len: box SZ.t)
+  (start_key_share: V.vec U8.t)
+  (start_cipher_suites: V.vec U16.t)
+  (start_cipher_suites_len: box SZ.t)
+  (start_signature_schemes: V.vec U16.t)
+  (start_signature_schemes_len: box SZ.t)
+  (client_hello_present: box bool)
+  (l: L.client_hello)
+  (client_hello_bytes: V.vec U8.t)
+  (client_hello_bytes_len: box SZ.t)
+  (network_out: array U8.t)
+  (network_out_len: SZ.t)
+  requires exists* random server_name server_name_len key_share
+                  cipher_suites cipher_suites_len
+                  signature_schemes signature_schemes_len
+                  old_present old_l_random old_l_server_name old_l_key_share
+                  old_l_cipher_suites old_l_signature_schemes
+                  old_client_hello_bytes_len old_client_hello_bytes old_network_out.
+          V.pts_to start_random random **
+          V.pts_to start_server_name server_name **
+          Box.pts_to start_server_name_len server_name_len **
+          V.pts_to start_key_share key_share **
+          V.pts_to start_cipher_suites cipher_suites **
+          Box.pts_to start_cipher_suites_len cipher_suites_len **
+          V.pts_to start_signature_schemes signature_schemes **
+          Box.pts_to start_signature_schemes_len signature_schemes_len **
+          Box.pts_to client_hello_present old_present **
+          V.pts_to l.L.client_hello_random old_l_random **
+          V.pts_to l.L.client_hello_server_name old_l_server_name **
+          V.pts_to l.L.client_hello_key_share old_l_key_share **
+          V.pts_to l.L.client_hello_cipher_suites old_l_cipher_suites **
+          V.pts_to l.L.client_hello_signature_schemes old_l_signature_schemes **
+          V.pts_to client_hello_bytes old_client_hello_bytes **
+          Box.pts_to client_hello_bytes_len old_client_hello_bytes_len **
+          pts_to network_out old_network_out **
+          pure (old_present == false /\
+                V.is_full_vec start_random /\
+                V.is_full_vec start_server_name /\
+                V.is_full_vec start_key_share /\
+                V.is_full_vec start_cipher_suites /\
+                V.is_full_vec start_signature_schemes /\
+                V.is_full_vec l.L.client_hello_random /\
+                V.is_full_vec l.L.client_hello_server_name /\
+                V.is_full_vec l.L.client_hello_key_share /\
+                V.is_full_vec l.L.client_hello_cipher_suites /\
+                V.is_full_vec l.L.client_hello_signature_schemes /\
+                V.is_full_vec client_hello_bytes /\
+                V.length start_random == 32 /\
+                V.length start_server_name == L.max_server_name_len /\
+                V.length start_key_share == 32 /\
+                V.length start_cipher_suites == L.max_cipher_suites /\
+                V.length start_signature_schemes == L.max_signature_schemes /\
+                V.length l.L.client_hello_random == 32 /\
+                V.length l.L.client_hello_server_name == L.max_server_name_len /\
+                V.length l.L.client_hello_key_share == 32 /\
+                V.length l.L.client_hello_cipher_suites == L.max_cipher_suites /\
+                V.length l.L.client_hello_signature_schemes == L.max_signature_schemes /\
+                V.length client_hello_bytes == 512 /\
+                B.length random == 32 /\
+                B.length server_name == L.max_server_name_len /\
+                B.length key_share == 32 /\
+                Seq.length cipher_suites == L.max_cipher_suites /\
+                Seq.length signature_schemes == L.max_signature_schemes /\
+                B.length old_l_random == 32 /\
+                B.length old_l_server_name == L.max_server_name_len /\
+                B.length old_l_key_share == 32 /\
+                Seq.length old_l_cipher_suites == L.max_cipher_suites /\
+                Seq.length old_l_signature_schemes == L.max_signature_schemes /\
+                B.length old_client_hello_bytes == 512 /\
+                B.length old_network_out == SZ.v network_out_len /\
+                517 <= SZ.v network_out_len /\
+                SZ.v server_name_len <= B.length server_name /\
+                SZ.v cipher_suites_len <= Seq.length cipher_suites /\
+                SZ.v signature_schemes_len <= Seq.length signature_schemes /\
+                Seq.equal random (Ghost.reveal start).CS.start_client_random /\
+                B.length (Ghost.reveal start).CS.start_server_name == SZ.v server_name_len /\
+                Seq.equal (Ghost.reveal start).CS.start_server_name (Seq.slice server_name 0 (SZ.v server_name_len)) /\
+                Seq.equal key_share (Ghost.reveal start).CS.start_client_key_share_public /\
+                L.cipher_suites_match
+                  cipher_suites
+                  (SZ.v cipher_suites_len)
+                  (Ghost.reveal start).CS.start_cipher_suites /\
+                L.signature_schemes_match
+                  signature_schemes
+                  (SZ.v signature_schemes_len)
+                  (Ghost.reveal start).CS.start_signature_schemes /\
+                Ghost.reveal ch == {
+                  M.random = (Ghost.reveal start).CS.start_client_random;
+                  M.server_name = Some (Ghost.reveal start).CS.start_server_name;
+                  M.key_share = (Ghost.reveal start).CS.start_client_key_share_public;
+                  M.cipher_suites = (Ghost.reveal start).CS.start_cipher_suites;
+                  M.signature_schemes = (Ghost.reveal start).CS.start_signature_schemes;
+                })
+  returns written: (n:SZ.t{SZ.v n <= SZ.v network_out_len})
+  ensures exists* random server_name server_name_len key_share
+                 cipher_suites cipher_suites_len
+                 signature_schemes signature_schemes_len
+                 handshake_bytes network_out_bytes handshake_len.
+          V.pts_to start_random random **
+          V.pts_to start_server_name server_name **
+          Box.pts_to start_server_name_len server_name_len **
+          V.pts_to start_key_share key_share **
+          V.pts_to start_cipher_suites cipher_suites **
+          Box.pts_to start_cipher_suites_len cipher_suites_len **
+          V.pts_to start_signature_schemes signature_schemes **
+          Box.pts_to start_signature_schemes_len signature_schemes_len **
+          Box.pts_to client_hello_present true **
+          V.pts_to l.L.client_hello_random random **
+          V.pts_to l.L.client_hello_server_name server_name **
+          V.pts_to l.L.client_hello_key_share key_share **
+          V.pts_to l.L.client_hello_cipher_suites cipher_suites **
+          V.pts_to l.L.client_hello_signature_schemes signature_schemes **
+          V.pts_to client_hello_bytes handshake_bytes **
+          Box.pts_to client_hello_bytes_len handshake_len **
+          pts_to network_out network_out_bytes **
+          pure (V.is_full_vec start_random /\
+               V.is_full_vec start_server_name /\
+               V.is_full_vec start_key_share /\
+               V.is_full_vec start_cipher_suites /\
+               V.is_full_vec start_signature_schemes /\
+               V.is_full_vec l.L.client_hello_random /\
+               V.is_full_vec l.L.client_hello_server_name /\
+               V.is_full_vec l.L.client_hello_key_share /\
+               V.is_full_vec l.L.client_hello_cipher_suites /\
+               V.is_full_vec l.L.client_hello_signature_schemes /\
+               V.is_full_vec client_hello_bytes /\
+               V.length start_random == 32 /\
+               V.length start_server_name == L.max_server_name_len /\
+               V.length start_key_share == 32 /\
+               V.length start_cipher_suites == L.max_cipher_suites /\
+               V.length start_signature_schemes == L.max_signature_schemes /\
+               V.length l.L.client_hello_random == 32 /\
+               V.length l.L.client_hello_server_name == L.max_server_name_len /\
+               V.length l.L.client_hello_key_share == 32 /\
+               V.length l.L.client_hello_cipher_suites == L.max_cipher_suites /\
+               V.length l.L.client_hello_signature_schemes == L.max_signature_schemes /\
+               V.length client_hello_bytes == 512 /\
+               B.length random == 32 /\
+               B.length server_name == L.max_server_name_len /\
+               B.length key_share == 32 /\
+               Seq.length cipher_suites == L.max_cipher_suites /\
+               Seq.length signature_schemes == L.max_signature_schemes /\
+               B.length handshake_bytes == 512 /\
+               B.length network_out_bytes == SZ.v network_out_len /\
+               SZ.v server_name_len <= B.length server_name /\
+               SZ.v cipher_suites_len <= Seq.length cipher_suites /\
+               SZ.v signature_schemes_len <= Seq.length signature_schemes /\
+               Seq.equal random (Ghost.reveal start).CS.start_client_random /\
+               B.length (Ghost.reveal start).CS.start_server_name == SZ.v server_name_len /\
+               Seq.equal (Ghost.reveal start).CS.start_server_name (CL.raw_slice server_name 0 (SZ.v server_name_len)) /\
+               Seq.equal key_share (Ghost.reveal start).CS.start_client_key_share_public /\
+               L.cipher_suites_match
+                 cipher_suites
+                 (SZ.v cipher_suites_len)
+                 (Ghost.reveal start).CS.start_cipher_suites /\
+               L.signature_schemes_match
+                 signature_schemes
+                 (SZ.v signature_schemes_len)
+                 (Ghost.reveal start).CS.start_signature_schemes /\
+               Seq.equal random (Ghost.reveal ch).M.random /\
+               L.optional_byte_prefix_matches
+                 true
+                 server_name
+                 server_name_len
+                 (Ghost.reveal ch).M.server_name /\
+               Seq.equal key_share (Ghost.reveal ch).M.key_share /\
+               L.cipher_suites_match
+                 cipher_suites
+                 (SZ.v cipher_suites_len)
+                 (Ghost.reveal ch).M.cipher_suites /\
+               L.signature_schemes_match
+                 signature_schemes
+                 (SZ.v signature_schemes_len)
+                 (Ghost.reveal ch).M.signature_schemes /\
+               SZ.v handshake_len == B.length (WS.serialize_handshake (M.ClientHello (Ghost.reveal ch))) /\
+               SZ.v handshake_len <= B.length handshake_bytes /\
+               Seq.equal
+                 (CL.raw_slice handshake_bytes 0 (SZ.v handshake_len))
+                 (WS.serialize_handshake (M.ClientHello (Ghost.reveal ch))) /\
+               SZ.v written ==
+                 B.length (CS.serialized_cleartext_tls_message (M.TlsHandshake (M.ClientHello (Ghost.reveal ch)))) /\
+               5 <= SZ.v written /\
+               SZ.v written <= B.length network_out_bytes /\
+               Seq.equal
+                 (CL.raw_slice network_out_bytes 0 (SZ.v written))
+                 (CS.serialized_cleartext_tls_message (M.TlsHandshake (M.ClientHello (Ghost.reveal ch)))) /\
+               CS.raw_records_exactly
+                 (CL.raw_slice network_out_bytes 0 (SZ.v written))
+                 T.Handshake
+                 1)
 
 fn encode_inner_plaintext_no_padding_slice
   (plain: array U8.t)
